rt refine: tune sched_context_relation; remove ADT_H sorry
The state relation was tracking the active refill list at the wrong
position (always assumed head). Haskell is tracking refills similarly
to C with indices into the Refill array (implemented as list), although
instead of head and tail, Haskell uses head and count.

The new formulation uses a map from Haskell to abstract, which can be
reused later in ADT_H.

Finally, this commit rephrases reply_stack_relation as a generic
heap_list relation, which has a generic proof of being functional.

All of these together + proof updated allow removal of the last sorry
in ADT_H.

Signed-off-by: Gerwin Klein <gerwin.klein@data61.csiro.au>

proof/refine/ARM/ADT_H.thy
@@ -12,6 +12,11 @@ imports
   Syscall_R
 begin
 
+(* FIXME: many of the naming conventions in this file are wrong. Definitions should start with
+          lower case letters, and should be under_score, not camelCase. Some, possibly many of
+          the functions here can benefit from projections that have been developed since this
+          was originally written *)
+
 text \<open>
   The general refinement calculus (see theory Simulation) requires
   the definition of a so-called ``abstract datatype'' for each refinement layer.
@@ -444,12 +449,33 @@ definition
       tcb_domain = tcbDomain tcb,
       tcb_arch = ArchTcbMap (tcbArch tcb)\<rparr>"
 
+definition absCNode :: "nat \<Rightarrow> (obj_ref \<rightharpoonup> kernel_object) \<Rightarrow> obj_ref \<Rightarrow> Structures_A.kernel_object"
+  where
+  "absCNode sz h a \<equiv> CNode sz (\<lambda>bl. if length bl = sz
+                                     then Some (CapabilityMap
+                                                  (case (h (a + of_bl bl * 2^cteSizeBits)) of
+                                                     Some (KOCTE cte) \<Rightarrow> cteCap cte))
+                                     else None)"
+
+definition scMap :: "(obj_ref \<rightharpoonup> obj_ref) \<Rightarrow> sched_context \<Rightarrow> Structures_A.sched_context" where
+  "scMap replyNexts sc = \<lparr>
+     sc_period     = scPeriod sc,
+     sc_budget     = scBudget sc,
+     sc_consumed   = scConsumed sc,
+     sc_tcb        = scTCB sc,
+     sc_ntfn       = scNtfn sc,
+     sc_refills    = refills_map (scRefillHead sc) (scRefillCount sc) (scRefillMax sc) (scRefills sc),
+     sc_refill_max = scRefillMax sc,
+     sc_badge      = scBadge sc,
+     sc_yield_from = scYieldFrom sc,
+     sc_replies    = heap_walk replyNexts (scReply sc) []
+   \<rparr>"
+
 definition
- "absCNode sz h a \<equiv> CNode sz (%bl.
-  if length bl = sz
-    then Some (CapabilityMap (case (h (a + of_bl bl * 2^cteSizeBits)) of
-                                Some (KOCTE cte) \<Rightarrow> cteCap cte))
-  else None)"
+  "mapScSize sc \<equiv> scBitsFromRefillLength' (length (scRefills sc)) - minSchedContextBits"
+
+definition replyMap :: "reply \<Rightarrow>  Structures_A.reply" where
+  "replyMap r = \<lparr> reply_tcb = replyTCB r, reply_sc = replySc r \<rparr>"
 
 definition
   absHeap :: "(word32 \<rightharpoonup> vmpage_size) \<Rightarrow> (word32 \<rightharpoonup> nat) \<Rightarrow>
@@ -464,6 +490,9 @@ definition
      | Some KOUserDataDevice \<Rightarrow> map_option (ArchObj \<circ> DataPage True) (ups x)
      | Some (KOTCB tcb) \<Rightarrow> Some (TCB (TcbMap tcb))
      | Some (KOCTE cte) \<Rightarrow> map_option (%sz. absCNode sz h x) (cns x)
+     | Some (KOReply reply) \<Rightarrow> Some (Structures_A.Reply (replyMap reply))
+     | Some (KOSchedContext sc) \<Rightarrow> Some (Structures_A.SchedContext
+                                           (scMap (h |> reply_of' |> replyNext_of) sc) (mapScSize sc))
      | Some (KOArch ako) \<Rightarrow> map_option ArchObj (absHeapArch h x ako)
      | None \<Rightarrow> None"
 
@@ -484,16 +513,6 @@ lemma unaligned_page_offsets_helper:
   apply clarsimp
   apply (case_tac vmpage_size, simp_all add: pageBits_def)
     apply (frule_tac i=n and k="0x1000" in word_mult_less_mono1, simp+)+
-  done
-
-(* FIXME: move *)
-lemma unaligned_helper:
-  "\<lbrakk>is_aligned x n; y\<noteq>0; y < 2 ^ n\<rbrakk> \<Longrightarrow> \<not> is_aligned (x + y) n"
-  apply (simp (no_asm_simp) add: is_aligned_mask)
-  apply (simp add: mask_add_aligned)
-  apply (cut_tac mask_eq_iff_w2p[of n y], simp_all add: word_size)
-  apply (rule ccontr)
-  apply (simp add: not_less power_overflow word_bits_conv)
   done
 
 lemma pspace_aligned_distinct_None:
@@ -576,15 +595,42 @@ lemma pspace_aligned_distinct_None':
    apply assumption+
   done
 
+lemma sc_replies_nexts_walk:
+  "\<lbrakk> sc_replies_relation s s';
+     ksPSpace s' p = Some (KOSchedContext sc'); kheap s p = Some (kernel_object.SchedContext sc n) \<rbrakk>
+   \<Longrightarrow> heap_walk (replyNexts_of s') (scReply sc') [] = sc_replies sc"
+  unfolding sc_replies_relation_def
+  apply (erule_tac x=p in allE)
+  apply (erule_tac x="sc_replies sc" in allE)
+  apply (clarsimp simp: sc_replies.all_simps)
+  apply (rule heap_list_is_walk)
+  apply (subgoal_tac "scReplies_of s' p = scReply sc'", simp)
+  apply (clarsimp simp: opt_map_def)
+  done
+
+context
+begin
+
+private method ako =
+  find_goal \<open>match premises in "kheap s p = Some (ArchObj ako)" for s p ako \<Rightarrow> succeed\<close>,
+  (rename_tac ako, case_tac ako;
+   clarsimp simp: other_obj_relation_def pte_relation_def pde_relation_def split: if_split_asm)
+
+private method ko =
+  case_tac ko; clarsimp simp: other_obj_relation_def cte_relation_def split: if_split_asm
+
+
 lemma absHeap_correct:
   assumes pspace_aligned:  "pspace_aligned s"
   assumes pspace_distinct: "pspace_distinct s"
   assumes valid_objs:      "valid_objs s"
   assumes pspace_relation: "pspace_relation (kheap s) (ksPSpace s')"
   assumes ghost_relation:  "ghost_relation (kheap s) (gsUserPages s') (gsCNodes s')"
+  assumes replies:         "sc_replies_relation s s'"
 shows
   "absHeap (gsUserPages s') (gsCNodes s') (ksPSpace s') = kheap s"
 proof -
+  note relatedE = pspace_dom_relatedE[OF _ pspace_relation]
   from ghost_relation
   have gsUserPages:
     "\<And>a sz. (\<exists>dev. kheap s a = Some (ArchObj (DataPage dev sz))) \<longleftrightarrow>
@@ -595,330 +641,265 @@ proof -
     by (fastforce simp add: ghost_relation_def)+
 
   show "?thesis"
-  supply  image_cong_simp [cong del]
+    supply image_cong_simp [cong del]
     apply (rule ext)
     apply (simp add: absHeap_def split: option.splits)
     apply (rule conjI)
      using pspace_relation
-     apply (clarsimp simp add: pspace_relation_def pspace_dom_def UNION_eq
-                               dom_def Collect_eq)
+     apply (clarsimp simp: pspace_relation_def pspace_dom_def UNION_eq dom_def Collect_eq)
      apply (erule_tac x=x in allE)
      apply clarsimp
      apply (case_tac "kheap s x", simp)
+     apply (rename_tac ko)
      apply (erule_tac x=x in allE, clarsimp)
      apply (erule_tac x=x in allE, simp add: Ball_def)
      apply (erule_tac x=x in allE, clarsimp)
 
-     apply (case_tac a)
-         apply (simp_all add: other_obj_relation_def
-                       split: if_split_asm Structures_H.kernel_object.splits)
+     apply (case_tac ko; simp add: other_obj_relation_def split: if_split_asm kernel_object.splits)
       apply (rename_tac sz cs)
-      apply (clarsimp simp add: image_def cte_map_def
-                 well_formed_cnode_n_def Collect_eq dom_def)
+      apply (clarsimp simp: image_def cte_map_def well_formed_cnode_n_def Collect_eq dom_def)
       apply (erule_tac x="replicate sz False" in allE)+
       apply simp
      apply (rename_tac arch_kernel_obj)
-     apply (case_tac arch_kernel_obj, simp_all add: image_def)
+     apply (case_tac arch_kernel_obj; simp add: image_def)
        apply (erule_tac x=0 in allE, simp)
       apply (erule_tac x=0 in allE, simp)
      apply clarsimp
      apply (erule_tac x=0 in allE, simp add: pageBits_def)
      apply (rename_tac vmpage_size)
-     apply (case_tac vmpage_size, simp_all)
+     apply (case_tac vmpage_size; simp)
 
-    apply clarsimp
+    apply (clarsimp split: kernel_object.splits)
     apply (intro conjI impI allI)
-           apply (erule pspace_dom_relatedE[OF _ pspace_relation])
-           apply clarsimp
-           apply (case_tac ko, simp_all add: other_obj_relation_def)
-             apply (clarsimp simp add: cte_relation_def split: if_split_asm)
-            apply (clarsimp simp add: ep_relation_def EndpointMap_def
-                     split: Structures_A.endpoint.splits)
-           apply (clarsimp simp add: EndpointMap_def
-                    split: Structures_A.endpoint.splits)
-  sorry (* FIXME RT: need map for SchedContexts
-           apply (rename_tac arch_kernel_obj)
-           apply (case_tac arch_kernel_obj,
-                  simp_all add: other_obj_relation_def)
-             apply (clarsimp simp add: pte_relation_def)
-            apply (clarsimp simp add: pde_relation_def)
-           apply (clarsimp split: if_split_asm)+
+             apply (erule relatedE, ko, ako)
+             apply (clarsimp simp: ep_relation_def EndpointMap_def
+                             split: Structures_A.endpoint.splits)
+            apply (erule relatedE, ko, ako)
+            apply (clarsimp simp: ntfn_relation_def NtfnMap_def
+                            split: Structures_A.ntfn.splits)
+           apply (erule relatedE, ko, ako)
+          apply (erule relatedE, ko, ako)
+          apply (rename_tac vmpage_size n)
+          apply (cut_tac a=y and sz=vmpage_size in gsUserPages, clarsimp split: if_split_asm)
+          apply (case_tac "n=0", simp)
+          apply (case_tac "kheap s (y + n * 2 ^ pageBits)")
+           apply (rule ccontr)
+           apply (clarsimp dest!: gsUserPages[symmetric, THEN iffD1] )
+          using pspace_aligned
+          apply (simp add: pspace_aligned_def dom_def)
+          apply (erule_tac x=y in allE)
+          apply (case_tac "n=0",(simp split: if_split_asm)+)
+          apply (frule (2) unaligned_page_offsets_helper)
+          apply (frule_tac y="n*2^pageBits" in pspace_aligned_distinct_None'
+                                            [OF pspace_aligned pspace_distinct])
+           apply simp
+           apply (rule conjI, clarsimp simp add: word_gt_0)
+           apply (simp add: is_aligned_mask)
+           apply (clarsimp simp add: pageBits_def mask_def)
+           apply (case_tac vmpage_size; frule_tac i=n and k="0x1000" in word_mult_less_mono1; simp)
+          apply simp
 
-          apply (erule pspace_dom_relatedE[OF _ pspace_relation])
-          apply (case_tac ko, simp_all add: other_obj_relation_def)
-            apply (clarsimp simp add: cte_relation_def split: if_split_asm)
-           apply (clarsimp simp add: ntfn_relation_def NtfnMap_def
-                    split: Structures_A.ntfn.splits)
-          apply (clarsimp simp add: NtfnMap_def
-                   split: Structures_A.ntfn.splits)
-          apply (rename_tac arch_kernel_obj)
-          apply (case_tac arch_kernel_obj, simp_all add: other_obj_relation_def)
-            apply (clarsimp simp add: pte_relation_def)
-           apply (clarsimp simp add: pde_relation_def)
-          apply (clarsimp split: if_split_asm)+
-
-         apply (erule pspace_dom_relatedE[OF _ pspace_relation])
-         apply (case_tac ko, simp_all add: other_obj_relation_def)
-           apply (clarsimp simp add: cte_relation_def split: if_split_asm)
-         apply (rename_tac arch_kernel_obj)
-         apply (case_tac arch_kernel_obj, simp_all add: other_obj_relation_def)
-           apply (clarsimp simp add: pte_relation_def)
-          apply (clarsimp simp add: pde_relation_def)
-         apply (clarsimp split: if_split_asm)+
-
-        apply (erule pspace_dom_relatedE[OF _ pspace_relation])
-        apply (case_tac ko, simp_all add: other_obj_relation_def)
-          apply (clarsimp simp add: cte_relation_def split: if_split_asm)
-        apply (rename_tac arch_kernel_obj)
-        apply (case_tac arch_kernel_obj, simp_all add: other_obj_relation_def)
-          apply (clarsimp simp add: pte_relation_def)
-         apply (clarsimp simp add: pde_relation_def)
-        apply (rename_tac vmpage_size)
-        apply (cut_tac a=y and sz=vmpage_size in gsUserPages, clarsimp split: if_split_asm)
-        apply (case_tac "n=0", simp)
-        apply (case_tac "kheap s (y + n * 2 ^ pageBits)")
-         apply (rule ccontr)
-         apply (clarsimp dest!: gsUserPages[symmetric, THEN iffD1] )
-        using pspace_aligned
-        apply (simp add: pspace_aligned_def dom_def)
-        apply (erule_tac x=y in allE)
-        apply (case_tac "n=0",(simp split: if_split_asm)+)
-        apply (frule (2) unaligned_page_offsets_helper)
-        apply (frule_tac y="n*2^pageBits" in pspace_aligned_distinct_None'
-                                          [OF pspace_aligned pspace_distinct])
+         apply (erule relatedE, ko, ako)
+         apply (rename_tac vmpage_size n)
+         apply (cut_tac a=y and sz=vmpage_size in gsUserPages, clarsimp split: if_split_asm)
+         apply (case_tac "n=0", simp)
+         apply (case_tac "kheap s (y + n * 2 ^ pageBits)")
+          apply (rule ccontr)
+          apply (clarsimp dest!: gsUserPages[symmetric, THEN iffD1])
+         using pspace_aligned
+         apply (simp add: pspace_aligned_def dom_def)
+         apply (erule_tac x=y in allE)
+         apply (case_tac "n=0"; simp)
+         apply (frule (2) unaligned_page_offsets_helper)
+         apply (frule_tac y="n*2^pageBits" in pspace_aligned_distinct_None'
+                                           [OF pspace_aligned pspace_distinct])
+          apply simp
+          apply (rule conjI, clarsimp simp add: word_gt_0)
+          apply (simp add: is_aligned_mask)
+          apply (clarsimp simp add: pageBits_def mask_def)
+          apply (case_tac vmpage_size; frule_tac i=n and k="0x1000" in word_mult_less_mono1; simp)
          apply simp
-         apply (rule conjI, clarsimp simp add: word_gt_0)
-         apply (simp add: is_aligned_mask)
-         apply (clarsimp simp add: pageBits_def mask_def)
-        apply (case_tac vmpage_size; simp)
-          apply ((frule_tac i=n and k="0x1000" in word_mult_less_mono1, simp+)+)[4]
-        apply (erule pspace_dom_relatedE[OF _ pspace_relation])
-        apply (case_tac ko, simp_all add: other_obj_relation_def)
-          apply (clarsimp simp add: cte_relation_def split: if_split_asm)
-        apply (rename_tac arch_kernel_obj)
-        apply (case_tac arch_kernel_obj, simp_all add: other_obj_relation_def)
-          apply (clarsimp simp add: pte_relation_def)
-         apply (clarsimp simp add: pde_relation_def)
-        apply (rename_tac vmpage_size)
-        apply (cut_tac a=y and sz=vmpage_size in gsUserPages, clarsimp split: if_split_asm)
-        apply (case_tac "n=0", simp)
-        apply (case_tac "kheap s (y + n * 2 ^ pageBits)")
-         apply (rule ccontr)
-         apply (clarsimp dest!: gsUserPages[symmetric, THEN iffD1])
-        using pspace_aligned
-        apply (simp add: pspace_aligned_def dom_def)
+
+        apply (erule relatedE, ko, ako)
+        apply (clarsimp simp: TcbMap_def tcb_relation_def valid_obj_def)
+        apply (rename_tac tcb y tcb')
+        apply (case_tac tcb, case_tac tcb')
+        apply (simp add: thread_state_relation_imp_ThStateMap)
+        apply (subgoal_tac "map_option FaultMap (tcbFault tcb) = tcb_fault")
+         prefer 2
+         apply (simp add: fault_rel_optionation_def)
+         using valid_objs[simplified valid_objs_def dom_def fun_app_def, simplified]
+         apply (erule_tac x=y in allE)
+         apply (clarsimp simp: valid_obj_def valid_tcb_def split: option.splits)
+        using valid_objs[simplified valid_objs_def Ball_def dom_def fun_app_def]
         apply (erule_tac x=y in allE)
-        apply (case_tac "n=0",simp+)
-        apply (frule (2) unaligned_page_offsets_helper)
-        apply (frule_tac y="n*2^pageBits" in pspace_aligned_distinct_None'
-                                          [OF pspace_aligned pspace_distinct])
+        apply (clarsimp simp: cap_relation_imp_CapabilityMap valid_obj_def valid_tcb_def
+                              ran_tcb_cap_cases valid_cap_def2 arch_tcb_relation_imp_ArchTcnMap)
+
+       apply (erule relatedE, ko, ako)
+       apply (simp add: absCNode_def cte_map_def)
+       apply (cut_tac a=y and n=sz in gsCNodes, clarsimp)
+       using pspace_aligned[simplified pspace_aligned_def]
+       apply (drule_tac x=y in bspec, clarsimp)
+       apply clarsimp
+       apply (case_tac "(of_bl ya::word32) * 2^cte_level_bits = 0", simp)
+        apply (rule ext)
+        apply simp
+        apply (rule conjI)
+         prefer 2
+         using valid_objs[simplified valid_objs_def Ball_def dom_def fun_app_def]
+         apply (erule_tac x=y in allE)
+         apply (clarsimp simp: valid_obj_def valid_cs_def valid_cs_size_def
+                               well_formed_cnode_n_def dom_def Collect_eq)
+         apply (frule_tac x=ya in spec, simp)
+         apply (erule_tac x=bl in allE)
+         apply clarsimp
+        apply (frule pspace_relation_absD[OF _ pspace_relation])
+        apply (simp add: cte_map_def)
+        apply (drule_tac x="y + of_bl bl * 2^cte_level_bits" in spec)
+        apply clarsimp
+        apply (erule_tac x="cte_relation bl" in allE)
+        apply (erule impE)
+         apply (fastforce simp add: well_formed_cnode_n_def)
+        apply clarsimp
+        apply (clarsimp simp add: cte_relation_def)
+        apply (rule cap_relation_imp_CapabilityMap)
+         using valid_objs[simplified valid_objs_def Ball_def dom_def fun_app_def]
+         apply (erule_tac x=y in allE)
+         apply (clarsimp simp: valid_obj_def valid_cs_def valid_cap_def2 ran_def)
+         apply (fastforce simp: cte_level_bits_def cteSizeBits_def)+
+       apply (subgoal_tac "kheap s (y + of_bl ya * 2^cte_level_bits) = None")
+        prefer 2
+        using valid_objs[simplified valid_objs_def Ball_def dom_def fun_app_def]
+        apply (erule_tac x=y in allE)
+        apply (clarsimp simp add: valid_obj_def valid_cs_def valid_cs_size_def)
+        apply (rule pspace_aligned_distinct_None'[OF
+                    pspace_aligned pspace_distinct], assumption)
+        apply (clarsimp simp: word_neq_0_conv power_add cte_index_repair)
+        apply (simp add: well_formed_cnode_n_def dom_def Collect_eq)
+        apply (erule_tac x=ya in allE)+
+        apply (rule word_mult_less_mono1)
+          apply (subgoal_tac "sz = length ya")
+           apply simp
+           apply (rule of_bl_length, (simp add: word_bits_def)+)[1]
+          apply fastforce
+         apply (simp add: cte_level_bits_def)
+        apply (simp add: word_bits_conv cte_level_bits_def)
+        apply (drule_tac a="2::nat" in power_strict_increasing, simp+)
+       apply (rule ccontr, clarsimp)
+       apply (cut_tac a="y + of_bl ya * 2^cte_level_bits" and n=yc in gsCNodes)
+       apply clarsimp
+
+      (* mapping architecture-specific objects *)
+      apply clarsimp
+      apply (rename_tac x arch_kernel_object)
+      apply (erule relatedE, ko)
+      apply (rename_tac y P arch_kernel_obj)
+      apply (case_tac arch_kernel_object; simp add: absHeapArch_def split: asidpool.splits)
+
+        apply clarsimp
+        apply (case_tac arch_kernel_obj)
+           apply (simp add: other_obj_relation_def asid_pool_relation_def inv_def o_def)
+          apply (clarsimp simp add:  pte_relation_def)
+         apply (clarsimp simp add:  pde_relation_def)
+        apply (clarsimp split: if_split_asm)+
+
+       apply (case_tac arch_kernel_obj)
+          apply (simp add: other_obj_relation_def asid_pool_relation_def inv_def o_def)
+         using pspace_aligned[simplified pspace_aligned_def Ball_def dom_def]
+         apply (erule_tac x=y in allE)
+         apply (clarsimp simp add: pte_relation_def absPageTable_def pt_bits_def pageBits_def)
+         apply (rule conjI)
+          prefer 2
+          apply clarsimp
+          apply (rule sym)
+          apply (rule pspace_aligned_distinct_None'[OF pspace_aligned pspace_distinct]; simp)
+          apply (cut_tac x=ya and n="2^10" in
+                 ucast_less_shiftl_helper[where 'a=32,simplified word_bits_conv]; simp)
+          apply (clarsimp simp add: word_gt_0)
+         apply clarsimp
+         apply (subgoal_tac "ucast ya << 2 = 0")
+          prefer 2
+          apply (rule ccontr)
+          apply (frule_tac x=y in unaligned_helper, assumption)
+           apply (rule ucast_less_shiftl_helper; simp)
+          apply simp
          apply simp
-         apply (rule conjI, clarsimp simp add: word_gt_0)
-         apply (simp add: is_aligned_mask)
-         apply (clarsimp simp add: pageBits_def mask_def)
-        apply (case_tac vmpage_size; simp)
-          apply ((frule_tac i=n and k="0x1000" in word_mult_less_mono1, simp+)+)[4]
-       apply (erule pspace_dom_relatedE[OF _ pspace_relation])
-       apply (case_tac ko, simp_all add: other_obj_relation_def)
-         apply (clarsimp simp add: cte_relation_def split: if_split_asm)
-        prefer 2
-        apply (rename_tac arch_kernel_obj)
-        apply (case_tac arch_kernel_obj, simp_all add: other_obj_relation_def)
-          apply (clarsimp simp add: pte_relation_def)
-         apply (clarsimp simp add: pde_relation_def)
-        apply (clarsimp split: if_split_asm)
-       apply (clarsimp simp add: TcbMap_def tcb_relation_def valid_obj_def)
-       apply (rename_tac tcb y tcb')
-       apply (case_tac tcb)
-       apply (case_tac tcb')
-       apply (simp add: thread_state_relation_imp_ThStateMap)
-       apply (subgoal_tac "map_option FaultMap (tcbFault tcb) = tcb_fault")
-        prefer 2
-        apply (simp add: fault_rel_optionation_def)
-        using valid_objs[simplified valid_objs_def dom_def fun_app_def,
-                         simplified]
-        apply (erule_tac x=y in allE)
-        apply (clarsimp simp: valid_obj_def valid_tcb_def
-                        split: option.splits)
-       using valid_objs[simplified valid_objs_def Ball_def dom_def fun_app_def]
-       apply (erule_tac x=y in allE)
-       apply (clarsimp simp add: cap_relation_imp_CapabilityMap valid_obj_def
-                                 valid_tcb_def ran_tcb_cap_cases valid_cap_def2
-                                 arch_tcb_relation_imp_ArchTcnMap)
-      apply (simp add: absCNode_def cte_map_def)
-      apply (erule pspace_dom_relatedE[OF _ pspace_relation])
-      apply (case_tac ko, simp_all add: other_obj_relation_def
-                                 split: if_split_asm)
-       prefer 2
-       apply (rename_tac arch_kernel_obj)
-       apply (case_tac arch_kernel_obj, simp_all add: other_obj_relation_def)
+         apply (rule ext)
+         apply (frule pspace_relation_absD[OF _ pspace_relation])
+         apply simp
+         apply (erule_tac x=offs in allE)
          apply (clarsimp simp add: pte_relation_def)
+         using valid_objs[simplified valid_objs_def fun_app_def dom_def, simplified]
+         apply (erule_tac x=y in allE)
+         apply (clarsimp simp add: valid_obj_def wellformed_pte_def)
+         apply (erule_tac x=offs in allE)
+         apply (rename_tac pte')
+         apply (case_tac pte', simp_all add: pte_relation_aligned_def)[1]
+          apply (clarsimp split: ARM_A.pte.splits)
+          apply (rule set_eqI, clarsimp)
+          apply (case_tac x; simp)
+         apply (clarsimp split: ARM_A.pte.splits)
+         apply (rule set_eqI, clarsimp)
+         apply (case_tac x; simp)
         apply (clarsimp simp add: pde_relation_def)
        apply (clarsimp split: if_split_asm)
-      apply (simp add: cte_map_def)
-      apply (clarsimp simp add: cte_relation_def)
-      apply (cut_tac a=y and n=sz in gsCNodes, clarsimp)
-      using pspace_aligned[simplified pspace_aligned_def]
-      apply (drule_tac x=y in bspec, clarsimp)
-      apply clarsimp
-      apply (case_tac "(of_bl ya::word32) * 2^cte_level_bits = 0", simp)
-       apply (rule ext)
-       apply simp
-       apply (rule conjI)
-        prefer 2
-        using valid_objs[simplified valid_objs_def Ball_def dom_def
-                                    fun_app_def]
-        apply (erule_tac x=y in allE)
-        apply (clarsimp simp add: valid_obj_def valid_cs_def valid_cs_size_def
-                    well_formed_cnode_n_def dom_def Collect_eq)
-        apply (frule_tac x=ya in spec, simp)
-        apply (erule_tac x=bl in allE)
-        apply clarsimp+
-       apply (frule pspace_relation_absD[OF _ pspace_relation])
-       apply (simp add: cte_map_def)
-       apply (drule_tac x="y + of_bl bl * 2^cte_level_bits" in spec)
-       apply clarsimp
-       apply (erule_tac x="cte_relation bl" in allE)
-       apply (erule impE)
-        apply (fastforce simp add: well_formed_cnode_n_def)
-       apply clarsimp
-       apply (clarsimp simp add: cte_relation_def)
-       apply (rule cap_relation_imp_CapabilityMap)
-        using valid_objs[simplified valid_objs_def Ball_def dom_def
-                                    fun_app_def]
-        apply (erule_tac x=y in allE)
-        apply (clarsimp simp: valid_obj_def valid_cs_def valid_cap_def2 ran_def)
-        apply (fastforce simp: cte_level_bits_def cteSizeBits_def)+
-      apply (subgoal_tac "kheap s (y + of_bl ya * 2^cte_level_bits) = None")
-       prefer 2
-       using valid_objs[simplified valid_objs_def Ball_def dom_def fun_app_def]
-       apply (erule_tac x=y in allE)
-       apply (clarsimp simp add: valid_obj_def valid_cs_def valid_cs_size_def)
-       apply (rule pspace_aligned_distinct_None'[OF
-                   pspace_aligned pspace_distinct], assumption)
-       apply (clarsimp simp: word_neq_0_conv power_add cte_index_repair)
-       apply (simp add: well_formed_cnode_n_def dom_def Collect_eq)
-       apply (erule_tac x=ya in allE)+
-       apply (rule word_mult_less_mono1)
-         apply (subgoal_tac "sz = length ya")
-          apply simp
-          apply (rule of_bl_length, (simp add: word_bits_def)+)[1]
-         apply fastforce
-        apply (simp add: cte_level_bits_def)
-       apply (simp add: word_bits_conv cte_level_bits_def)
-       apply (drule_tac a="2::nat" in power_strict_increasing, simp+)
-      apply (rule ccontr, clarsimp)
-      apply (cut_tac a="y + of_bl ya * 2^cte_level_bits" and n=yc in gsCNodes)
-      apply clarsimp
 
-    (* mapping architecture-specific objects *)
-    apply clarsimp
-    apply (erule pspace_dom_relatedE[OF _ pspace_relation])
-    apply (case_tac ko, simp_all add: other_obj_relation_def)
-     apply (clarsimp simp add: cte_relation_def split: if_split_asm)
-    apply (rename_tac arch_kernel_object y ko P arch_kernel_obj)
-    apply (case_tac arch_kernel_object, simp_all add: absHeapArch_def
-                                            split: asidpool.splits)
-
-      apply clarsimp
       apply (case_tac arch_kernel_obj)
-         apply (simp add: other_obj_relation_def asid_pool_relation_def
-                          inv_def o_def)
+         apply (simp add: other_obj_relation_def asid_pool_relation_def inv_def o_def)
         apply (clarsimp simp add:  pte_relation_def)
-       apply (clarsimp simp add:  pde_relation_def)
-      apply (clarsimp split: if_split_asm)+
-
-     apply (case_tac arch_kernel_obj)
-        apply (simp add: other_obj_relation_def asid_pool_relation_def inv_def
-                         o_def)
-       using pspace_aligned[simplified pspace_aligned_def Ball_def dom_def]
+       using pspace_aligned
+       apply (simp add: pspace_aligned_def dom_def)
        apply (erule_tac x=y in allE)
-       apply (clarsimp simp add: pte_relation_def absPageTable_def
-                                 pt_bits_def pageBits_def)
+       apply (clarsimp simp add: pde_relation_def absPageDirectory_def pd_bits_def pageBits_def)
        apply (rule conjI)
         prefer 2
         apply clarsimp
         apply (rule sym)
-        apply (rule pspace_aligned_distinct_None'
-                    [OF pspace_aligned pspace_distinct], simp+)
-        apply (cut_tac x=ya and n="2^10" in
-               ucast_less_shiftl_helper[where 'a=32,simplified word_bits_conv], simp+)
+        apply (rule pspace_aligned_distinct_None' [OF pspace_aligned pspace_distinct]; simp)
+        apply (cut_tac x=ya and n="2^14" in
+               ucast_less_shiftl_helper[where 'a=32, simplified word_bits_conv]; simp)
         apply (clarsimp simp add: word_gt_0)
        apply clarsimp
        apply (subgoal_tac "ucast ya << 2 = 0")
         prefer 2
         apply (rule ccontr)
         apply (frule_tac x=y in unaligned_helper, assumption)
-         apply (rule ucast_less_shiftl_helper, simp_all)
+         apply (rule ucast_less_shiftl_helper; simp)
+        apply simp
+       apply simp
        apply (rule ext)
        apply (frule pspace_relation_absD[OF _ pspace_relation])
        apply simp
        apply (erule_tac x=offs in allE)
-       apply (clarsimp simp add: pte_relation_def)
-       using valid_objs[simplified valid_objs_def fun_app_def dom_def,
-                        simplified]
+       apply (clarsimp simp add: pde_relation_def)
+
+       using valid_objs[simplified valid_objs_def fun_app_def dom_def,simplified]
        apply (erule_tac x=y in allE)
-       apply (clarsimp simp add: valid_obj_def wellformed_pte_def)
+       apply (clarsimp simp add: valid_obj_def wellformed_pde_def)
        apply (erule_tac x=offs in allE)
-       apply (rename_tac pte')
-       apply (case_tac pte', simp_all add: pte_relation_aligned_def)[1]
-        apply (clarsimp split: ARM_A.pte.splits)
+       apply (rename_tac pde')
+       apply (case_tac pde'; simp add: pde_relation_aligned_def)
+          apply (clarsimp split: ARM_A.pde.splits)+
+         apply (fastforce simp add: subset_eq)
+        apply (clarsimp split: ARM_A.pde.splits)
         apply (rule set_eqI, clarsimp)
-        apply (case_tac x, simp_all)[1]
-       apply (clarsimp split: ARM_A.pte.splits)
+        apply (case_tac x; simp)
+       apply (clarsimp split: ARM_A.pde.splits)
        apply (rule set_eqI, clarsimp)
-       apply (case_tac x, simp_all)[1]
-      apply (clarsimp simp add: pde_relation_def)
-     apply (clarsimp split: if_split_asm)+
+       apply (case_tac x; simp)
+      apply (clarsimp simp add: pde_relation_def split: if_split_asm)
 
-    apply (case_tac arch_kernel_obj)
-       apply (simp add: other_obj_relation_def asid_pool_relation_def inv_def
-                        o_def)
-      apply (clarsimp simp add:  pte_relation_def)
-     using pspace_aligned
-     apply (simp add: pspace_aligned_def dom_def)
-     apply (erule_tac x=y in allE)
-     apply (clarsimp simp add: pde_relation_def absPageDirectory_def
-                               pd_bits_def pageBits_def)
-     apply (rule conjI)
-      prefer 2
-      apply clarsimp
-      apply (rule sym)
-      apply (rule pspace_aligned_distinct_None'
-                  [OF pspace_aligned pspace_distinct], simp+)
-      apply (cut_tac x=ya and n="2^14" in
-             ucast_less_shiftl_helper[where 'a=32, simplified word_bits_conv], simp+)
-      apply (clarsimp simp add: word_gt_0)
-     apply clarsimp
-     apply (subgoal_tac "ucast ya << 2 = 0")
-      prefer 2
-      apply (rule ccontr)
-      apply (frule_tac x=y in unaligned_helper, assumption)
-       apply (rule ucast_less_shiftl_helper, simp_all)
-     apply (rule ext)
-     apply (frule pspace_relation_absD[OF _ pspace_relation])
-     apply simp
-     apply (erule_tac x=offs in allE)
-     apply (clarsimp simp add: pde_relation_def)
+     apply (rule relatedE, assumption, ko, ako)
+     apply (frule scBits_inverse_sc_relation)
+     apply (clarsimp simp: sc_relation_def scMap_def mapScSize_def sc_replies_nexts_walk[OF replies])
 
-     using valid_objs[simplified valid_objs_def fun_app_def dom_def,simplified]
-     apply (erule_tac x=y in allE)
-     apply (clarsimp simp add: valid_obj_def wellformed_pde_def)
-     apply (erule_tac x=offs in allE)
-     apply (rename_tac pde')
-     apply (case_tac pde', simp_all add: pde_relation_aligned_def)[1]
-        apply (clarsimp split: ARM_A.pde.splits)+
-       apply (fastforce simp add: subset_eq)
-      apply (clarsimp split: ARM_A.pde.splits)
-      apply (rule set_eqI, clarsimp)
-      apply (case_tac x, simp_all)[1]
-     apply (clarsimp split: ARM_A.pde.splits)
-     apply (rule set_eqI, clarsimp)
-     apply (case_tac x, simp_all)[1]
-    apply (clarsimp simp add: pde_relation_def split: if_split_asm)
-    done *)
+    apply (erule relatedE, ko, ako)
+    apply (clarsimp simp: reply_relation_def replyMap_def)
+    done
 qed
 
+end
 
 text \<open>The following function can be used to reverse cte_map.\<close>
 definition
@@ -989,12 +970,11 @@ lemma TCB_implies_KOTCB:
 lemma cte_at_CNodeI:
   "\<lbrakk>kheap s a = Some (CNode (length b) cs); well_formed_cnode_n (length b) cs\<rbrakk>
    \<Longrightarrow> cte_at (a,b) s"
-apply (subgoal_tac "\<exists>y. cs b = Some y")
- apply clarsimp
- apply (rule_tac cte=y in cte_wp_at_cteI[of s _ "length b" cs],
-        simp_all)
-apply (simp add: well_formed_cnode_n_def dom_def Collect_eq)
-done
+  apply (subgoal_tac "\<exists>y. cs b = Some y")
+   apply clarsimp
+   apply (rule_tac cte=y in cte_wp_at_cteI[of s _ "length b" cs]; simp)
+  apply (simp add: well_formed_cnode_n_def dom_def Collect_eq)
+  done
 
 lemma cteMap_correct:
   assumes rel:              "(s,s') \<in> state_relation"
